changing has_type const_t to be like var_t

src/Typing.v
@@ -24,7 +24,8 @@ Inductive term : Set :=
 (** * Syntax-directed rule system of Damas-Milner *)
 
 Inductive has_type : ctx -> term -> ty -> Prop :=
-| const_ht : forall x i G, in_ctx x G = Some (sc_con i) -> has_type G (const_t x) (con i)
+| const_ht : forall x G sigma tau, in_ctx x G = Some sigma -> is_schm_instance tau sigma ->
+                            has_type G (const_t x) tau
 | var_ht : forall x G sigma tau, in_ctx x G = Some sigma -> is_schm_instance tau sigma ->
                             has_type G (var_t x) tau
 | lam_ht : forall x G tau tau' e, has_type ((x, ty_to_schm tau) :: G) e tau' ->
@@ -98,15 +99,20 @@ Proof.
   - intros. inversion H. subst. rewrite apply_subst_arrow.
     econstructor. rewrite <- ty_to_subst_schm. rewrite apply_subst_ctx_eq. apply IHe.
     assumption.
-  - intros. inversion H. subst. rewrite apply_subst_con.
+  - intros. inversion H.
+    subst.
     econstructor.
     + induction G; simpl in *; mysimp.
       destruct a.
       mysimp.
-      rewrite apply_subst_schm_con.
-      reflexivity.
       apply IHG.
       econstructor.
+      apply H1.
       assumption.
       assumption.
+    + unfold is_schm_instance in *.
+      destruct H3.
+      eapply subst_inst_subst_type in H0.
+      exists (map_apply_subst_ty s x).
+      apply H0.
 Qed.
